{
 "cells": [
  {
   "cell_type": "code",
   "execution_count": null,
   "id": "c095671b-09aa-4f05-aefd-464ffcc59b8f",
   "metadata": {},
   "outputs": [],
   "source": [
    "1. Find the value of T(2) for the recurrence relation T(n) = 3T(n-1) + 12n, given that T(0)=5.\n"
   ]
  },
  {
   "cell_type": "code",
   "execution_count": null,
   "id": "6b2506e3-8dcb-4da0-95d6-40da0ab9effa",
   "metadata": {},
   "outputs": [],
   "source": [
    "Recurrence Relation\n",
    "𝑇(𝑛)=3𝑇(𝑛−1)+12𝑛\n",
    "\n",
    "Given \n",
    "T(0)=5.\n",
    "\n",
    "n=1,   \n",
    "𝑇(1)= 3𝑇(0) + 12⋅1\n",
    "𝑇(1)=3 ⋅5 + 12\n",
    "T(1)= 15 + 12 \n",
    "T(1)= 27\n",
    "\n",
    "n=2,\n",
    "T(2)= 3T(1) + 12⋅2\n",
    "T(2)= 3⋅27 + 24 \n",
    "T(2)= 81 + 24 \n",
    "𝑇(2)= 105\n",
    "\n",
    "The value of T(2) is 105\n"
   ]
  },
  {
   "cell_type": "code",
   "execution_count": null,
   "id": "d2d4cf68-3166-438d-a2df-7e0c4468a080",
   "metadata": {},
   "outputs": [],
   "source": [
    "2. Given a recurrence relation, solve it using the substitution method:\n",
    "a. T(n) = T(n-1) + c\n",
    "b. T(n) = 2T(n/2) + n\n",
    "c. T(n) = 2T(n/2) + c\n",
    "d. T(n) = T(n/2) + c"
   ]
  },
  {
   "cell_type": "code",
   "execution_count": null,
   "id": "ce93f2a1-2cc1-4577-b141-e503daea6d74",
   "metadata": {},
   "outputs": [],
   "source": [
    "To solve recurrence relations using the substitution method, we make an educated guess (or hypothesis) about the form of the \n",
    "solution and then use mathematical induction to prove it. Here’s how you can approach each of the given recurrence relations:\n",
    "\n",
    "### a.  T(n) = T(n-1) + c \n",
    "\n",
    "**Hypothesis:** Let  T(n) = an + b .\n",
    "\n",
    "Substitute into the recurrence relation:\n",
    "\n",
    " Assume  T(n) = an + b \n",
    " Substitute into the recurrence relation:\n",
    "   T(n) = T(n-1) + c\n",
    "   T(n) = a(n-1) + b + c\n",
    "   T(n) = an - a + b + c\n",
    "   an - a + b + c = an + b\n",
    "   \n",
    " Solving for a  and  b:\n",
    "   -a + c = 0 implies a = c\n",
    "\n",
    "   b is the constant term and remains b.\n",
    "\n",
    "Solution:\n",
    "    T(n) = cn + b\n",
    "   \n",
    "   Given the initial condition \n",
    "                 T(0)=T 0, we find 𝑏=𝑇0\n",
    "\n",
    "General Solution:\n",
    "   T(n) = cn + T0\n",
    "\n",
    "\n",
    "\n",
    "### b.  T(n) = 2T(n/2) + n \n",
    "\n",
    "Hypothesis: Let T(n)= anlogn + b. \n",
    "\n",
    "Substitute into the recurrence relation:\n",
    "\n",
    "Assume T(n)= anlogn+b\n",
    "T(n) = 2[ a(n/2 log n/2)+b]+ n\n",
    "T(n) = an log n/2 + 2b + n\n",
    "T(n) = an(logn−log2)+2b+n\n",
    "T(n) = anlogn−anlog2+2b+n\n",
    "\n",
    "To match the original form T(n)=anlogn+b, we need\n",
    "      −alog2+1 = 0\n",
    "⟹    a = 1 /log2\n",
    "      b = 2b− an log2\n",
    "To simplify, we use a=1, b=constant.\n",
    "\n",
    "Solution:\n",
    "​\n",
    "   T(n) = nlogn + O(n)\n",
    "\n",
    "\n",
    "\n",
    "c. T(n)=2T(n/2)+c\n",
    "Hypothesis: Let T(n)=anlogn+b.\n",
    "\n",
    "Substitute into the recurrence relation:\n",
    "\n",
    "Assume T(n)=anlogn+b.\n",
    "Substitute into the recurrence relation:\n",
    "\n",
    "T(n)=2T(n/2)+c\n",
    "\n",
    "T(n)=2[a( 2nlog 2n)+b]+c\n",
    "\n",
    "T(n)=an log 2n+2b+c\n",
    "\n",
    "T(n)=an(logn−log2)+2b+c\n",
    "\n",
    "T(n)=anlogn−anlog2+2b+c\n",
    "\n",
    "To match the original form T(n)=anlogn+b, \n",
    "   we get:   a=a\n",
    "\n",
    "  b=2b−anlog2+c\n",
    "\n",
    "To match:\n",
    "a=2, b=c\n",
    "\n",
    "Solution:\n",
    "\n",
    "  T(n) = Θ(nlogn)\n",
    "\n",
    "\n",
    "\n",
    "\n",
    "### d.  T(n) = T(n/2) + c \n",
    "\n",
    " Assume  T(n) = a log n + b \n",
    " Substitute into the recurrence relation:\n",
    "   \n",
    "   T(n) = a log n/2 +b +c\n",
    "   T(n) = a(log n- log2) +b +c\n",
    "   T(n) = alogn - alog2 +b+c\n",
    "\n",
    "To match the original form   T(n)=alogn+b:\n",
    "                                a = a\n",
    "                                b = −alog2+b+c\n",
    "                                −alog2 + c = 0\n",
    "\n",
    "\n",
    "Solving gives a=constant.\n",
    "\n",
    "Solution:\n",
    "\n",
    " T(n) = Θ(logn)\n"
   ]
  },
  {
   "cell_type": "code",
   "execution_count": null,
   "id": "9819f2a0-2d9b-49ab-bd03-7d2f6b2cea55",
   "metadata": {},
   "outputs": [],
   "source": [
    "3. Given a recurrence relation, solve it using the recursive tree approach:\n",
    "a. T(n) = 2T(n-1) +1\n",
    "b. T(n) = 2T(n/2) + n"
   ]
  },
  {
   "cell_type": "code",
   "execution_count": null,
   "id": "c5289516-ed4d-4cf7-a19e-b536df2ee13f",
   "metadata": {},
   "outputs": [],
   "source": [
    "Recursive Tree Approach:\n",
    "\n",
    "a.   Draw the Recursive Tree:\n",
    "\n",
    "At the root (level 0), we have T(n).\n",
    "At level 1, this splits into two subproblems: \n",
    "\n",
    "T(n−1) and T(n−1), with an additional cost of 1.\n",
    "At level 2, each T(n−1) further splits into \n",
    "2×T(n−2) with an additional cost of 1, and so on.\n",
    "\n",
    " Cost at Each Level:\n",
    "\n",
    "Level 0: Cost = 1\n",
    "Level 1: Cost = 2\n",
    "Level 2: Cost = 4\n",
    "...\n",
    "Level k: Cost = 2^k\n",
    "\n",
    "The total cost at each level doubles as we go down the tree. The depth of the tree is n since the smallest problem we can get to is \n",
    "T(1), which implies the tree has n levels.\n",
    "\n",
    "Total Cost Calculation:\n",
    "\n",
    "Sum the costs across all levels:\n",
    "\n",
    "Total Cost = 1+2+4+⋯+2^n−1\n",
    "This is a geometric series with the sum:\n",
    "Total Cost = 2^n -1 \n",
    "T(n) grows as 2^n, so the time complexity is O(2^n)\n",
    "​\n",
    "\n",
    "b. T(n)=2T(n/2)+n  \n",
    "\n",
    "Draw the Recursive Tree:\n",
    "\n",
    "At the root (level 0), we have T(n).\n",
    "At level 1, this splits into two subproblems:  T(n/2) and T(n/2), with an additional cost of 𝑛\n",
    "At level 2, each T(n/2) further splits into T(n/4), and so on.\n",
    "\n",
    "Cost at Each Level:\n",
    "\n",
    "Level 0: Cost = 𝑛\n",
    "Level 1: Cost = 2× 𝑛/2 = 𝑛\n",
    "Level 2: Cost = 4× 𝑛/4 = 𝑛\n",
    "Level k: Cost = 𝑛\n",
    "\n",
    "The cost at each level remains 𝑛 and the tree has log 𝑛 levels because the problem size halves at each level until it reaches 1.\n",
    "\n",
    "Total Cost Calculation:\n",
    "\n",
    "Sum the costs across all levels:\n",
    "\n",
    "Total Cost=n+n+n+⋯+n(logn times)\n",
    "Total Cost=n×logn"
   ]
  }
 ],
 "metadata": {
  "kernelspec": {
   "display_name": "Python 3 (ipykernel)",
   "language": "python",
   "name": "python3"
  },
  "language_info": {
   "codemirror_mode": {
    "name": "ipython",
    "version": 3
   },
   "file_extension": ".py",
   "mimetype": "text/x-python",
   "name": "python",
   "nbconvert_exporter": "python",
   "pygments_lexer": "ipython3",
   "version": "3.11.5"
  }
 },
 "nbformat": 4,
 "nbformat_minor": 5
}
